\levelstaynon{10.3.2 - Distribution of the time to reach a certain distance}

\leveldownnon{Problem}

The problem has three parts:
\begin{enumerate}[\indent a.]
  \item Consider the problem of diffusion on the interval $[-a, a]$ with absorbing boundary conditions. Use the survival probability from Eq.~(8.8) to find the first passage time probability density to hit the boundaries.
  \item Find the mean first-passage time to hit the boundaries.
  \item Define $\Delta g \equiv \left( \baravg{t^2} - (\baravg{t})^2 \right)$. Compute the quantity $\Delta t / \baravg{t}$.
\end{enumerate}


\levelstaynon{Solution}

The survival probability density is
\begin{equation*}
  S(t) = \frac{4}{\pi} \sum_{n=0}^\infty \frac{(-1)^n}{2n + 1} \exp \left(
    - \frac{(2n + 1)^2 \pi^2 D t}{4 a ^2}
  \right)
\end{equation*}
so the first-passage time density to the boundaries is
\begin{align*}
  q(\pm a, t | 0)
  &= - \left( \frac{dS}{dt} \right)(t) \\
  &= \frac{\pi D}{a^2} \sum_{n=0}^\infty (-1)^n (2 n + 1) \exp \left(
    - \frac{(2n + 1)^2 \pi^2 D t}{4 a ^2}
  \right)
\end{align*}
which solves \textbf{part a}.
For \textbf{part b} we use the generating function
\begin{equation*}
  \tilde{q}(\pm a, s | 0)
  = \frac{\pi D}{a^2} \sum_{n=0}^\infty (-1)^n (2n + 1) \left( s + \frac{(2n + 1)^2 \pi^2 D}{4 a^2} \right)^{-1}
  \, .
\end{equation*}
Its derivative is
\begin{align*}
  \left(- \frac{d \tilde{q}}{ds} \right)(\pm a, s | 0)
  &= \frac{\pi D}{a^2} \sum_{n=0}^\infty (-1)^n (2n + 1)
    \left( s + \frac{(2n + 1)^2 \pi^2 D}{4 a^2} \right)^{-2} \\
  \baravg{t(0 \rightarrow \pm a)} = \left(- \frac{d \tilde{q}}{ds} \right)(\pm a, s=0 | 0)
  &= \frac{\pi D}{a^2} \sum_{n=0}^\infty (-1)^n (2n + 1)
    \left( \frac{(2n + 1)^2 \pi^2 D}{4 a^2} \right)^{-2} \\
  &= \frac{\pi D (4a^2)^2}{a^2 (\pi^2 D)^2} \underbrace{\sum_{n=0}^\infty (-1)^n (2n + 1)^{-3}}_{\pi^3 / 32} \\
  &= \frac{a^2}{2 D}
  \, .
\end{align*}
Finally, for \textbf{part c}, we compute the second moment of the first-passage time.
We do this again using the generating function.
\begin{align*}
  \frac{d^2 q}{ds^2}
  &= \frac{\pi D}{a^2} \sum_{n=0}^\infty (-1)^n (2n + 1) (-1)(-2)
    \left( s + \frac{(2n + 1)^2 \pi^2 D}{4 a^2} \right)^{-3} \\
  \baravg{t^2}
  = \left( \frac{d^2 q}{ds^2} \right)(\pm a, s=0 | 0)
  &= \frac{2 \pi D (4a^2)^3}{a^2 (\pi^2 D)^3} \underbrace{\sum_{n=0}^\infty (-1)^n (2n + 1)^{-5}}_{5 \pi^5 / 1536} \\
  &= \frac{2^7 a^4}{\pi^5 D^2} \frac{5 \pi^5}{12 \cdot 2^7} \\
  &= \frac{5}{12} \left( \frac{a^2}{D} \right)^2
  \, .
\end{align*}
Therefore
\begin{align*}
  \Delta t
  &= \left( \baravg{t^2} - (\baravg{t})^2 \right)^{1/2} \\
  &= \frac{a^2}{D} \left( \frac{5}{12} - \frac{1}{4} \right)^{1/2} \\
  &= \frac{1}{\sqrt{6}} \frac{a^2}{D}
\end{align*}
and finally $\Delta t / \baravg{t} = 2 / \sqrt{6} = \sqrt{2 / 3}$, which agrees with Balki.
