\levelstay{Problem 7.5.5 (AO)}
\textbf{(a):} The $l^{th}$ moment of the radial distance is given by
\begin{eqnarray}
\overline{r^l(t)} &=& \int_{0}^{\infty} \text{p}_\text{rad}(r, t) r^l dr \nonumber \\
&=&  \int_{0}^{\infty} \frac{1}{(4 \pi D t)^{3/2}} 4 \pi r^2 \exp(-r^2/4Dt) r^l dr \nonumber \\
&=&  \int_{0}^{\infty} \frac{1}{(4 \pi D t)^{3/2}} 4 \pi (4 D t z) \exp(-z) (4 D t z)^{l/2} \frac{(4 D t)^{1/2} ~dz}{2 (z)^{1/2}} \nonumber \\
&=&  \frac{2}{\sqrt{\pi}} \int_{0}^{\infty} \frac{(4 D t)^{1+l/2+1/2}}{(4 D t)^{3/2}}~ z^{1+l/2-1/2} \exp(-z) dz \nonumber \\
&=& \frac{2^{l+1}}{\sqrt{\pi}} (D t)^{l/2} \int_{0}^{\infty}~ z^{(l+1)/2} \exp(-z) dz \nonumber \\
&=& \boxed{\frac{2^{l+1}}{\sqrt{\pi}} (D t)^{l/2}~\Gamma\bigg(\frac{1}{2}(l+3)\bigg)}~.
\end{eqnarray}
Note that when $l$ is odd, the argument of the $\Gamma$-function is an integer. As $\Gamma(n+1) = n!$ for all $n \geq 0 $, it follows that 
\begin{equation}
\boxed{ \overline{r^l(t)} = \frac{2^{l+1}}{\sqrt{\pi}} (D t)^{l/2} ([l+1]/2)!~~\text{when}~l~\text{is odd.}} \label{eq:odd_radial_moments}
\end{equation}

When $l$ is even, the argument of the $\Gamma$-function is equal to an integer plus a half. Using the equation (see Appendix B of the textbook)
\begin{equation}
\Gamma(n+1/2) = \frac{\sqrt{\pi} (2n-1)!}{2^{2n-1}(n-1)!}~\text{for}~n = 1, 2, \ldots \nonumber
\end{equation}
and equating $(l+3)/2 = n + 1/2$ leaves us with
\begin{eqnarray}
\overline{r^l(t)} &=& \frac{2^{l+1}}{\sqrt{\pi}} (D t)^{l/2} \frac{\sqrt{\pi} (l+2-1)!}{2^{l+2-1}((l+2)/2-1)!} \nonumber \\
&=& \boxed{(D t)^{l/2} \frac{(l+1)!}{(l/2)!} ~~\text{when}~l~\text{is even.}} \label{eq:even_radial_moments}
\end{eqnarray}

\textbf{(b):} The $l=-1$ can be deduced from Eq. (\ref{eq:odd_radial_moments}) as $\Gamma(1) = 0! = 1$ is defined. From here it follows that $\overline{r^{-1}(t)} = 1/\sqrt{\pi Dt}$. The $l=-2$ moment cannot be derived from equation Eq. (\ref{eq:even_radial_moments}); however, the problem boils down to a simple Gaussian integral as shown below:
\begin{eqnarray}
\overline{r^{-2}(t)} &=& \int_{0}^{\infty} \frac{1}{(4 \pi D t)^{3/2}} 4 \pi r^2 \exp(-r^2/4Dt) r^{-2} dr \nonumber \\
&=& \frac{4 \pi \sqrt{4Dt}}{\pi^{3/2} (4Dt)^{3/2}} \times \int_{0}^{\infty} \underbrace{\exp(-z^2) dz}_{=\sqrt{\pi}/2} \nonumber \\
&=& \boxed{\frac{1}{2Dt}}~.
\end{eqnarray}
