\levelstay{Problem 7.5.2 (AO)}
\textbf{(a):} Show that, if $p(x,0)=p_\text{init}(x)$, then
\begin{equation}
p(x,t) = \int_{-\infty}^{\infty} dx_0~G(x, t; x_0, 0)~p_\text{init}(x_0).
\end{equation}

Repeating the calculation from problem 7.1 with $p(x,~t=0) = p_\text{init}(x)$ yields
\begin{equation}
\tilde{p}(k, s)  = \frac{\tilde{p}(k, 0)}{s + D k^2}
\end{equation}
which implies that 
\begin{equation}
\mathcal{L}^{-1} [\tilde{p}(k, s)] = \tilde{p}(k, t) = \exp(-D k^2 t) \cdot \tilde{p}(k, 0).
\end{equation}
Taking the inverse Fourier transform of this equation gives us
\begin{eqnarray}
\mathcal{F}^{-1} [\tilde{p}(k, t)] &=& p(x,t) \nonumber \\
&=& \int_{-\infty}^{\infty} dx_0~ G(x-x_0,~t;~0,~0)~p(x_0,0) \nonumber \\
&=& \int_{-\infty}^{\infty} dx_0~ G(x,~t;~x_0,~0)~p(x_0,0) \nonumber \\
&=& \boxed{\int_{-\infty}^{\infty} dx_0~G(x,~t;~x_0,~0)~p_\text{init}(x_0)}~.
\end{eqnarray}

\textbf{(b):} Assuming $p_\text{init}(x)$ is an even function of $x$, show that $p(x,t)$ is also an even function of $x$.

Starting with the equation 
\begin{equation}
p(x,t) = \int_{-\infty}^{\infty} dx_0~\frac{1}{\sqrt{4 \pi D t} } \exp\bigg(- \frac{(x-x_0)^2}{4 D t}\bigg)~p_\text{init}(x_0),
\end{equation}
let's evaluate this expression under the subsitution $x \rightarrow -x$, which gives us
\begin{equation}
p(-x,t) = \int_{-\infty}^{\infty} dx_0~\frac{1}{\sqrt{4 \pi D t} } \exp\bigg(- \frac{(-x-x_0)^2}{4 D t}\bigg)~p_\text{init}(x_0).
\end{equation}
Making the change of variables $x_0' = -x_0$, we have that
\begin{eqnarray}
p(-x,t) &=& \int_{\infty}^{-\infty} -dx_0'~\frac{1}{\sqrt{4 \pi D t} } \exp\bigg(- \frac{(-x+x_0')^2}{4 D t}\bigg)~p_\text{init}(-x_0') \nonumber \\
&=& \int_{-\infty}^{\infty} dx_0'~\frac{1}{\sqrt{4 \pi D t} } \exp\bigg(- \frac{(-x+x_0')^2}{4 D t}\bigg)~p_\text{init}(-x_0') \nonumber \\
&=& \int_{-\infty}^{\infty} dx_0'~\frac{1}{\sqrt{4 \pi D t} } \exp\bigg(- \frac{(x-x_0')^2}{4 D t}\bigg)~p_\text{init}(-x_0') \nonumber \\
&=& \int_{-\infty}^{\infty} dx_0'~\frac{1}{\sqrt{4 \pi D t} } \exp\bigg(- \frac{(x-x_0')^2}{4 D t}\bigg)~p_\text{init}(x_0') \nonumber \\
&=& p(x,t),
\end{eqnarray}
where the second to last line follows from the fact that $p_\text{init}(x_0)$ is even.